spec/DNS.Protocol.Parser.EverParseRuntime.fsti
@@ -260,6 +260,8 @@ val check_dns_uncompressed_question_srv_answer_packet :
 val check_dns_uncompressed_question_compressed_srv_answer_packet :
   qname_length:FStar.UInt32.t ->
   rr_name_length:FStar.UInt32.t ->
+  target_name_ptr_hi_value:FStar.UInt32.t ->
+  target_name_ptr_lo_value:FStar.UInt32.t ->
   base:buffer FStar.UInt8.t ->
   len:FStar.UInt32.t ->
   Stack bool
